#信息论 

>[!NOTE]
>$h(a X)$:
>$$
\begin{gathered}
\boldsymbol{h}(\boldsymbol{a X})=\boldsymbol{h}(\boldsymbol{X})+\log |\boldsymbol{a}| \\
\boldsymbol{h}(\boldsymbol{A X})=\boldsymbol{h}(\boldsymbol{X})+\log |\operatorname{det} \boldsymbol{A}|
\end{gathered}
>$$
>Let $Y=a X$. Then according to:  $$f_{Y}(y)dy=\sum f_{x}(x_{i})dx$$
>Where $x_{i}$ are the roots of $y=x$ .
>
>$f_Y(y)=\frac{1}{|a|} f_X\left(\frac{y}{a}\right)$, and
>$$
>\begin{aligned}
>h(a X) & =-\int f_Y(y) \log f_Y(y) d y \\
>& =-\int \frac{1}{|a|} f_X\left(\frac{y}{a}\right) \log \left(\frac{1}{|a|} f_X\left(\frac{y}{a}\right)\right) d y \\
>& =-\int f_X(x) \log f_X(x) d x+\log |a| \\
>& =h(X)+\log |a|
>\end{aligned}
>$$
>$$
>\boldsymbol{h}(\boldsymbol{A} \boldsymbol{X})=\boldsymbol{h}(\boldsymbol{X})+\log |\operatorname{det}(\boldsymbol{A})|
>$$
